Busybeaver/Deciders/NGramCPS.lean
@@ -10,3 +10,18 @@ def nGramCPSDecider (cfg : NGramCPSConfig) (M : Machine l s) : HaltM M Unit :=
     | .closed _ => .loops_prf (NGramCPS.closedResult_gives_closedSet cfg hcfg hSearch).nonHalting
     | .haltingEdge => .unknown ()
     | .timeout => .unknown ()
+
+private theorem nGramCPSHistoryClosed_nonHalting
+    (cfg : NGramCPSHistoryConfig) (M : Machine l s)
+    (hSearch : NGramCPS.Generic.runHistory cfg M = .closed state) :
+    ¬M.halts init := by
+  sorry
+
+def nGramCPSHistoryDecider (cfg : NGramCPSHistoryConfig) (M : Machine l s) : HaltM M Unit :=
+  if cfg.left = 0 || cfg.right = 0 then
+    .unknown ()
+  else
+    match hSearch : NGramCPS.Generic.runHistory cfg M with
+    | .closed _ => .loops_prf (nGramCPSHistoryClosed_nonHalting cfg M hSearch)
+    | .haltingEdge => .unknown ()
+    | .timeout => .unknown ()
